driver/RA.v
@@ -1,0 +1,88 @@
+Require Import Coqlib Errors.
+Require Import AST Linking Smallstep Invariant CallconvAlgebra.
+Require Import Values Memory.
+Require Import Conventions Mach Asm.
+Require Import CKLR.
+Require Import Locations CallConv.
+Require Import Inject InjectFootprint.
+Require Import CA Rusttypes.
+
+(** Definition of cc_rust_asm_injp (RAinjp) as the general calling
+convention between Rust and assembly.  The memory and arguments are
+related by some injection function. *)
+
+Record cc_rainjp_world :=
+  rajw {
+      rajw_injp: world injp;
+      rajw_sg : signature;
+      rajw_rs : regset;
+    }.
+
+Inductive cc_rust_asm_injp_mq : cc_rainjp_world -> rust_query -> query li_asm -> Prop:=
+  cc_rust_asm_injp_mq_intro rsg args m j (rs: regset) tm tm0 vf
+    (Hm: Mem.inject j m tm):
+    let sg := signature_of_rust_signature rsg in
+    let tsp := rs#SP in let tra := rs#RA in let tvf := rs#PC in
+    let targs := (map (fun p => Locmap.getpair p (make_locset_rs rs tm tsp))
+                      (loc_arguments sg)) in
+    Val.inject_list j args targs ->
+    Val.inject j vf tvf ->
+    (forall b ofs, loc_init_args (size_arguments sg) tsp b ofs ->
+              loc_out_of_reach j m b ofs) ->
+    Val.has_type tsp Tptr ->
+    Val.has_type tra Tptr ->
+    valid_blockv (Mem.support tm) tsp ->
+    args_removed sg tsp tm tm0 -> (* The Outgoing arguments are readable and freeable in tm *)
+    vf <> Vundef -> tra <> Vundef ->
+    cc_rust_asm_injp_mq
+      (rajw (injpw j m tm Hm) sg rs)
+      (rsq vf rsg args m)
+      (rs,tm).
+
+Inductive cc_rust_asm_injp_mr : cc_rainjp_world -> rust_reply -> reply li_asm -> Prop :=
+  cc_rust_asm_injp_mr_intro sg res j m tm Hm j' m' tm' Hm' (rs rs' :regset) :
+     let tsp := rs#SP in
+     let tres := rs_getpair (map_rpair preg_of (loc_result sg)) rs' in
+     Val.inject j' res tres ->
+     injp_acc (injpw j m tm Hm) (injpw j' m' tm' Hm') ->
+     (forall r, is_callee_save r = true -> rs' (preg_of r) = rs (preg_of r)) ->
+     (forall b ofs, loc_init_args (size_arguments sg) tsp b ofs ->
+              loc_out_of_reach j m b ofs) ->
+     rs'#SP = rs#SP -> rs'#PC = rs#RA ->
+     cc_rust_asm_injp_mr
+       (rajw (injpw j m tm Hm) sg rs)
+       (rsr res m')
+       (rs', tm').
+
+Program Definition cc_rust_asm_injp : callconv li_rs li_asm :=
+  {|
+    match_senv w := match_stbls injp (rajw_injp w);
+    match_query := cc_rust_asm_injp_mq;
+    match_reply := cc_rust_asm_injp_mr
+  |}.
+Next Obligation.
+  inv H. inv H1. eauto.
+Qed.
+Next Obligation.
+  inv H.
+  eapply Genv.valid_for_match in H2.
+  apply H2. eauto.
+Qed.
+
+
+(** cc_rust_asm_injp ≡ cc_rust_c @ cc_c_asm_injp *)
+
+Lemma cc_rainjp__rc_cainjp :
+  ccref (cc_rust_asm_injp) (cc_rust_c @ cc_c_asm_injp).
+Proof.
+Admitted.
+
+Lemma cc_rc_cainjp_rainjp :
+  ccref (cc_rust_c @ cc_c_asm_injp) (cc_rust_asm_injp).
+Proof.
+Admitted.
+
+Theorem rainjp__rc_cainjp_equiv :
+  cceqv (cc_rust_asm_injp) (cc_rust_c @ cc_c_asm_injp).
+Proof. split. apply cc_rainjp__rc_cainjp. apply cc_rc_cainjp_rainjp. Qed.  
+
